coqimp/framework/soundness/soundness.v
@@ -23,17 +23,73 @@ Definition ins_sound p q i :=
   forall s,
     s |= p -> (exists s', (Q__ s (cntrans i) s') /\ s' |= q).
 
-(*
-Inductive safety : nat -> CodeHeap -> State -> Label -> Label -> asrt -> nat -> Prop :=
-| safety_ret1 :
-     forall C S S1 S2 pc pc1 pc2 npc npc1 npc2 q,
+Inductive comtype := tc | ti | tj | tr | tbe | tbne.
+
+Inductive steprecord :=
+| step_end : steprecord
+| step_cons : comtype -> steprecord -> steprecord.
+
+Inductive safety_step : CodeHeap -> State -> Label -> Label -> asrt -> steprecord -> nat -> Prop :=
+| safety_step_i :
+    forall C S pc npc q n cls,
+      (forall S' i pc' npc', 
+        C pc = Some (cntrans i) ->
+        P__ C (S, pc, npc) (S', pc', npc') ->
+        safety_step C S' pc' npc' q cls n) ->
+      safety_step C S pc npc q (step_cons ti cls) n
+
+| safety_step_j :
+    forall C S pc npc q n cls,
+      (forall S1 S2 pc1 pc2 npc1 npc2 aexp rd,
+        C pc = Some (cjumpl aexp rd) ->
+        P__ C (S, pc, npc) (S1, pc1, npc1) ->
+        P__ C (S1, pc1, npc1) (S2, pc2, npc2) ->
+        safety_step C S2 pc2 npc2 q cls n) ->
+      safety_step C S pc npc q (step_cons tj cls) n
+
+| safety_step_be :
+    forall C S pc npc q n cls,
+      (forall S1 S2 pc1 pc2 npc1 npc2 aexp,
+        C pc = Some (cbe aexp) ->
+        P__ C (S, pc, npc) (S1, pc1, npc1) ->
+        P__ C (S1, pc1, npc1) (S2, pc2, npc2) ->
+        safety_step C S2 pc2 npc2 q cls n) ->
+      safety_step C S pc npc q (step_cons tbe cls) n
+
+| safety_step_bne :
+    forall C S pc npc q n cls,
+      (forall S1 S2 pc1 pc2 npc1 npc2 aexp,
+        C pc = Some (cbne aexp) ->
+        P__ C (S, pc, npc) (S1, pc1, npc1) ->
+        P__ C (S1, pc1, npc1) (S2, pc2, npc2) ->
+        safety_step C S2 pc2 npc2 q cls n) ->
+      safety_step C S pc npc q (step_cons tbne cls) n
+
+| safety_step_call :
+    forall C S pc npc q n cls,
+      (forall S1 S2 pc1 pc2 npc1 npc2 f,
+        C pc = Some (ccall f) ->
+        P__ C (S, pc, npc) (S1, pc1, npc1) ->
+        P__ C (S1, pc1, npc1) (S2, pc2, npc2) ->
+        safety_step C S2 pc2 npc2 q cls (Nat.succ n)) ->
+      safety_step C S pc npc q (step_cons tc cls) n
+
+| safety_step_ret1 :
+    forall C S pc npc q,
+      (forall S1 S2 pc1 pc2 npc1 npc2,
         C pc = Some (cretl) ->
         P__ C (S, pc, npc) (S1, pc1, npc1) ->
-        P__ C (S1, pc1, npc1) (S2, pc2, npc2) -> S2 |= q ->
-        safety 2 C S pc npc q 0
+        P__ C (S1, pc1, npc1) (S2, pc2, npc2) -> S2 |= q) ->
+      safety_step C S pc npc q (step_end) 0
 
-               | 
-*)
+| safety_step_ret2 :
+    forall C S pc npc q n cls,
+      (forall S1 S2 pc1 pc2 npc1 npc2,
+        C pc = Some (cretl) ->
+        P__ C (S, pc, npc) (S1, pc1, npc1) ->
+        P__ C (S1, pc1, npc1) (S2, pc2, npc2) ->
+        safety_step C S2 pc2 npc2 q cls n) ->
+      safety_step C S pc npc q (step_cons tr cls) (Nat.succ n).        
 
 (*+ soundness of instruction rule +*)
 CoInductive safety : CodeHeap -> State -> Label -> Label -> asrt -> nat -> Prop :=
