coqimp/framework/soundness/wfcdhp_sound.v
@@ -1,8 +1,8 @@
-Require Import Coqlib.  
-Require Import Maps. 
+Require Import Coqlib.   
+Require Import Maps.  
 Require Import LibTactics.
-
-Require Import Integers.
+   
+Require Import Integers. 
 Open Scope Z_scope.  
 Import ListNotations.
 
@@ -265,6 +265,50 @@ Proof.
   eauto.
 Qed.
 
+Lemma exe_delay_general_reg_stable :
+  forall D R R' D' (r : GenReg),
+    exe_delay R D = (R', D') ->
+    (forall v, R r = Some v <-> R' r = Some v).
+Proof.
+  intro D.
+  induction D; intros.
+  -
+    simpls.
+    inversion H; subst.
+    split; eauto.
+
+  -
+    destruct a, p.
+    simpl in H.
+    destruct d.
+    {
+      destruct (exe_delay R D) eqn:Heqe.
+      inversion H; subst.
+      eapply IHD in Heqe; eauto.
+      split.
+      intro.
+      eapply Heqe in H0.
+      unfold set_R.
+      unfold is_indom.
+      destruct (r0 s) eqn:Heqe1; eauto.
+      unfold RegMap.set.
+      destruct_rneq.
+      intro.
+      eapply Heqe; eauto.
+      clear - H0.
+      unfolds set_R.
+      unfold is_indom in *.
+      destruct (r0 s) eqn:Heqe; tryfalse; tryfalse; eauto.
+      unfolds RegMap.set.
+      destruct_rneq_H.
+    }
+    {
+      destruct (exe_delay R D) eqn:Heqe.
+      inversion H; subst.
+      eapply IHD in Heqe; eauto.
+    }
+Qed.
+    
 (*+ Lemmas for expression +*)
 Lemma eval_addrexp_merge_still :
   forall M m aexp l,
@@ -730,6 +774,17 @@ Proof.
   inversion H; get_ins_diff_false.
   eauto.
 Qed.
+
+Lemma pc_bne_npc_i :
+  forall pc npc C aexp I,
+    LookupC C pc npc I ->
+    C pc = Some (cbne aexp) ->
+    exists i, C npc = Some (cntrans i).
+Proof.
+  intros.
+  inversion H; get_ins_diff_false.
+  eauto.
+Qed.
   
 (*+ progress +*)
 Lemma seq_progress :
@@ -1132,9 +1187,9 @@ Proof.
     eapply H1 in H12.
     simpljoin1.
     destruct (Int.eq bv ($ 0)) eqn:Heqe.
-    { 
+    {   
       exists (m, (R', f0), D') x f2 (f2 +ᵢ ($ 4)) (f2 +ᵢ ($ 4)) ((f2 +ᵢ ($ 4)) +ᵢ ($ 4)).
-      split.
+      split. 
       econstructor; eauto.
       eapply Be_false; eauto.
       eapply H2 in H9.
@@ -1160,9 +1215,416 @@ Proof.
       econstructor; eauto.
       eapply NTrans; eauto.
     }
+    {
+      exists (m, (R', f0), D') x f2 f f (f +ᵢ ($ 4)).
+      split.
+      econstructor; eauto.
+      eapply Be_true; eauto.
+      instantiate (1 := bv).
+      eapply H2 in H9.
+      clear - H9.
+      sep_star_split_tac.
+      simpl in H3.
+      simpljoin1.
+      simpl in H1.
+      unfolds regSt.
+      simpls.
+      simpljoin1.
+      unfold merge.
+      unfold RegMap.set.
+      destruct_rneq.
+      clear - Heqe.
+      unfolds Int.eq.
+      intro.
+      destruct (zeq (Int.unsigned bv) (Int.unsigned $ 0)) eqn:Heqe1; tryfalse.
+      destruct_state x.
+      econstructor; eauto.
+      eapply NTrans; eauto.
+    }
+
+  -
+    clear H4.
+    sep_star_split_tac.
+    simpl in H9.
+    simpljoin1.
+    eapply IHwf_seq in H1; eauto.
+    simpljoin1.
+    destruct_state x.
+    destruct_state x0. 
+    eapply program_step_safety_property with (s := (merge m m0, (merge r0 r1, f0), d0))
+      in H1; eauto.
+    simpljoin1.
+    destruct_state x0.
+    simpl in H10.
+    simpljoin1.
+    eapply program_step_safety_property with (s := (merge m1 m3, (merge r2 r4, f2), d2))
+      in H9; eauto.
+    simpljoin1.
+    destruct_state x0.
+    simpl in H13.
+    simpljoin1. 
+    exists (m1 ⊎ m3, (r2 ⊎ r4, f2), d2) (m2 ⊎ m4, (r3 ⊎ r5, f), d)
+      x1 x2 x3 x4.
+   split; eauto.
+   simpl; eauto.
+   simpl; eauto.
+
+  -
+    simpl in H1.
+    simpljoin1.
+    eauto.
+
+  -
+    eapply H0 in H2.
+    eauto.
+Qed.
+
+Lemma bne_progress :
+  forall p q S pc npc aexp C Spec I,
+    wf_seq Spec p I q -> LookupC C pc npc I -> S |= p ->
+    C pc = Some (cbne aexp) ->
+    exists S1 S2 pc1 pc2 npc1 npc2,
+      P__ C (S, pc, npc) (S1, pc1, npc1) /\
+      P__ C (S1, pc1, npc1) (S2, pc2, npc2).
+Proof.
+  intros.
+  generalize dependent C.
+  generalize dependent S.
+  generalize dependent pc.
+  generalize dependent npc.
+  generalize dependent aexp.
+
+  induction H; intros; elim_ins_neq.
+
+  -
+    clear H15.
+    destruct_state S.
+    assert (Hexe_dly1 : exists R' D', exe_delay r0 d = (R', D')).
+    {
+      eapply exe_delay_no_abort; eauto.
+    }
+    simpljoin1.
+    renames x to R', x0 to D'.
+    lets Hexe_delay1 : H9.
+    symmetry in H9.
+    eapply dly_reduce_asrt_stable in H9; eauto.
+    lets Haexp : H9.
+    eapply H in Haexp.
+    simpl in Haexp.
+    simpljoin1.
+    assert (Hexe_delay2 : exists R'' D'', exe_delay R' D' = (R'', D'')).
+    {
+      eapply exe_delay_no_abort; eauto.
+    }
+    simpljoin1.
+    renames x to R'', x0 to D''.
+    lets Hexe_delay2 : H12.
+    symmetry in H12.
+    eapply dly_reduce_asrt_stable in H12; eauto.
+    eapply ins_rule_sound in H1.
+    eapply H1 in H12.
+    simpljoin1.
+    destruct (Int.eq bv ($ 0)) eqn:Heqe.
+    { 
+      exists (m, (R', f0), D') x f2 f f (f +ᵢ ($ 4)).
+      split.  
+      econstructor; eauto.
+      eapply Bne_true; eauto.
+      eapply H2 in H9.
+      clear - H9 Heqe.
+      sep_star_split_tac.
+      simpls.
+      simpljoin1.
+      unfolds regSt.
+      simpls.
+      simpljoin1.
+      unfold merge.
+      unfold RegMap.set.
+      destruct_rneq.
+      clear - Heqe.
+      unfolds Int.eq.
+      destruct (zeq (Int.unsigned bv) (Int.unsigned $ 0)); tryfalse.
+      eapply z_eq_to_int_eq in e; eauto.
+      do 2 rewrite Int.repr_unsigned in e.
+      subst.
+      eauto.
+      destruct_state x.
+      econstructor; eauto.
+      eapply NTrans; eauto.
+    }
+    {
+      exists (m, (R', f0), D') x f2 (f2 +ᵢ ($ 4)) (f2 +ᵢ ($ 4)) ((f2 +ᵢ ($ 4)) +ᵢ ($ 4)).
+      split.
+      econstructor; eauto.
+      eapply Bne_false; eauto.
+      instantiate (1 := bv).
+      eapply H2 in H9.
+      clear - H9 Heqe.
+      simpl in H9.
+      unfolds regSt.
+      simpls.
+      simpljoin1.
+      destruct_state x.
+      destruct_state x0.
+      simpls.
+      simpljoin1.
+      unfold merge.
+      unfold RegMap.set.
+      destruct_rneq.
+      clear - Heqe.
+      unfolds Int.eq.
+      destruct (zeq (Int.unsigned bv) (Int.unsigned $ 0)); tryfalse.
+      intro.
+      subst.
+      eapply n.
+      simpl; eauto.
+      destruct_state x. 
+      econstructor; eauto.
+      eapply NTrans; eauto.
+    }
+
+  -
+    clear H4.
+    sep_star_split_tac.
+    simpl in H9.
+    simpljoin1.
+    eapply IHwf_seq in H1; eauto.
+    simpljoin1.
+    destruct_state x.
+    destruct_state x0. 
+    eapply program_step_safety_property with (s := (merge m m0, (merge r0 r1, f0), d0))
+      in H1; eauto.
+    simpljoin1.
+    destruct_state x0.
+    simpl in H10.
+    simpljoin1.
+    eapply program_step_safety_property with (s := (merge m1 m3, (merge r2 r4, f2), d2))
+      in H9; eauto.
+    simpljoin1.
+    destruct_state x0.
+    simpl in H13.
+    simpljoin1. 
+    exists (m1 ⊎ m3, (r2 ⊎ r4, f2), d2) (m2 ⊎ m4, (r3 ⊎ r5, f), d)
+      x1 x2 x3 x4.
+   split; eauto.
+   simpl; eauto.
+   simpl; eauto.
+
+  -
+    simpl in H1.
+    simpljoin1.
+    eauto.
+
+  -
+    eapply H0 in H2.
+    eauto.
+Qed.
+
+Lemma retl_progress :
+  forall p q S pc npc C I Spec,
+    wf_seq Spec p I q -> LookupC C pc npc I -> S |= p ->
+    C pc = Some (cretl) ->
+    exists S1 S2 pc1 pc2 npc1 npc2,
+      P__ C (S, pc, npc) (S1, pc1, npc1) /\
+      P__ C (S1, pc1, npc1) (S2, pc2, npc2).
+Proof.
+  intros.
+  generalize dependent C.
+  generalize dependent S.
+  generalize dependent pc.
+  generalize dependent npc.
+
+  induction H; intros; elim_ins_neq.
+
+  - 
+    clear H10.
+    destruct_state S.
+    assert (Hexe_dly1 : exists R' D', exe_delay r d = (R', D')).
+    {
+      eapply exe_delay_no_abort; eauto.
+    }
+    simpljoin1.
+    renames x to R', x0 to D'.
+    lets Hexe_delay1 : H5.
+    symmetry in H5.
+    eapply dly_reduce_asrt_stable in H5; eauto.
+    assert (Hexe_dly2 : exists R'' D'', exe_delay R' D' = (R'', D'')).
+    {
+      eapply exe_delay_no_abort; eauto.
+    }
+    simpljoin1.
+    renames x to R'', x0 to D''.
+    lets Hexe_delay2 : H6.
+    symmetry in H6.
+    eapply dly_reduce_asrt_stable in H6; eauto.
+    eapply ins_rule_sound in H.
+    lets Hp' : H6.
+    eapply H in Hp'; eauto.
+    simpljoin1.
+    destruct_state x.
+    unfolds fretSta.
+    lets Hret_f : H6.
+    eapply H1 in Hret_f; eauto.
+    simpljoin1.
+    simpls.  
+    exists (m, (R', f), D') (m0, (r0, f0), d0) f2 (x +ᵢ ($ 8)) (x +ᵢ ($ 8)) (x +ᵢ ($ 12)).
+    split. 
+    econstructor; eauto.
+    eapply Retl; eauto.
+    eapply exe_delay_general_reg_stable in H9; eauto.
+    econstructor; eauto.
+    assert (x +ᵢ ($ 12) = (x +ᵢ ($ 8)) +ᵢ ($ 4)).
+    {
+      rewrite Int.add_assoc; eauto.
+    }
+    rewrite H11; eauto.
+    eapply NTrans; eauto.
+
+  -
+    sep_star_split_tac.
+    simpl in H9.
+    simpljoin1.
+    eapply IHwf_seq in H1; eauto.
+    simpljoin1.
+    destruct_state x.
+    destruct_state x0.
+    eapply program_step_safety_property with (s := (merge m m0, (merge r0 r1, f0), d0))
+      in H1; eauto.
+    simpljoin1.
+    destruct_state x0.
+    simpl in H9.
+    simpljoin1.
+    eapply program_step_safety_property with (s := (merge m1 m3, (merge r2 r4, f2), d2))
+      in H7; eauto.
+    simpljoin1.
+    exists (m1 ⊎ m3, (r2 ⊎ r4, f2), d2) x x1 x2 x3 x4.
+    split; eauto.
+    simpl; eauto.
+    simpl; eauto.
+
+  -
+    simpl in H1.
+    simpljoin1.
+    eauto.
+
+  -
+    eapply H0 in H2.
+    eauto.
+Qed.
+
+Lemma call_progress :
+  forall p q S pc npc C I Spec f,
+    wf_seq Spec p I q -> LookupC C pc npc I -> S |= p ->
+    C pc = Some (ccall f) ->
+    exists S1 S2 pc1 pc2 npc1 npc2,
+      P__ C (S, pc, npc) (S1, pc1, npc1) /\
+      P__ C (S1, pc1, npc1) (S2, pc2, npc2).
+Proof.
+  intros.
+  generalize dependent C.
+  generalize dependent S.
+  generalize dependent pc.
+  generalize dependent npc.
+
+  induction H; intros; elim_ins_neq.
+
+  -
+    clear H18.
+    destruct_state S.
+    assert (Hexe_dly1 : exists R' D', exe_delay r0 d = (R', D')).
+    {
+      eapply exe_delay_no_abort; eauto.
+    }
+    simpljoin1.
+    renames x to R', x0 to D'.
+    lets Hexe_delay1 : H11.
+    symmetry in H11.
+    eapply dly_reduce_asrt_stable in H11; eauto.
+    lets Hr15 : H11.
+    eapply H0 in Hr15.
+    assert (Hr15' : (m, (set_R R' r15 f1, f), D') |= r15 |=> f1 ** p1).
+    {
+      clear - Hr15.
+      sep_star_split_tac.
+      simpls.
+      simpljoin1.
+      unfolds regSt.
+      simpls.
+      simpljoin1.
+      exists (empM, (set_R (RegMap.set r15 (Some v) empR) r15 f1, f2), d0)
+        (m1, (r0, f2), d0).
+      simpls.
+      repeat (split; eauto).
+      eapply disjoint_setR_still1; eauto.
+      rewrite indom_setR_merge_eq1; eauto.
+      eapply regset_l_l_indom; eauto.
+      rewrite indom_setR_eq_RegMap_set; eauto.
+      rewrite regset_twice; eauto.
+      eapply regset_l_l_indom; eauto.
+    }
     
-    >>>>>>>
-    
+    assert (Hexe_dly2 : exists R'' D'', exe_delay (set_R R' r15 f1) D' = (R'', D'')).
+    {
+      eapply exe_delay_no_abort; eauto.
+    }
+    simpljoin1.
+    renames x to R'', x0 to D''.
+    lets Hexe_delay2 : H12.
+    symmetry in H12. 
+    eapply dly_reduce_asrt_stable in H12; eauto.
+    eapply ins_rule_sound in H1.
+    eapply H1 in H12.
+    simpljoin1.  
+    exists (m, (set_R R' r15 f1, f), D') x (f1 +ᵢ ($ 4)) f0 f0 (f0 +ᵢ ($ 4)).
+    split.
+    econstructor; eauto.
+    eapply Call; eauto.
+    clear - Hr15.
+    sep_star_split_tac.
+    simpls.
+    simpljoin1.
+    unfolds regSt.
+    simpls.
+    simpljoin1.
+    eapply indom_merge_still; eauto.
+    eapply regset_l_l_indom; eauto.
+    destruct_state x.
+    econstructor; eauto.
+    eapply NTrans; eauto.
+
+  -
+    sep_star_split_tac.
+    simpls.
+    simpljoin1.
+    eapply IHwf_seq in H1; eauto.
+    simpljoin1.
+    destruct_state x.
+    destruct_state x0.
+    eapply program_step_safety_property with (s := (merge m m0, (merge r0 r1, f1), d0))
+      in H1; eauto.
+    simpljoin1.
+    destruct_state x0.
+    simpls.
+    simpljoin1.
+    eapply program_step_safety_property with (s := (merge m1 m3, (merge r2 r4, f3), d2))
+      in H8; eauto.
+    simpljoin1.
+    destruct_state x0.
+    simpls.
+    simpljoin1.
+    exists (m1 ⊎ m3, (r2 ⊎ r4, f3), d2) (m2 ⊎ m4, (r3 ⊎ r5, f), d) x1 x2 x3 x4.
+    split; eauto.
+    simpl; eauto.
+    simpl; eauto.
+
+  -
+    simpls.
+    simpljoin1.
+    eauto.
+
+  -
+    eauto.
+Qed.
     
 (*+ preservation +*)
 Lemma seq_preservation :
@@ -1715,8 +2177,447 @@ Proof.
     rewrite H5 in H9.
     inversion H9; subst.
     clear H9 H10.
-    >>>>>>>>>>>>>>>>>>>>>>>
+    sep_star_split_tac.
+    simpl in H13.
+    simpljoin1.
+    eapply be_progress in H; eauto.
+    simpljoin1.
+    destruct_state x.
+    destruct_state x0.
+    eapply IHwf_seq in H1; eauto.
+    destruct H1 as [ I' [p' H1] ].
+    simpljoin1. 
+    eapply program_step_safety_property with (s := (merge m m0, (merge r0 r1, f0), d0)) (r := r)
+      in H; eauto.
+    simpljoin1.
+    destruct_state x0.
+    simpl in H16.
+    simpljoin1.
+    eapply program_step_safety_property with (s := (merge m1 m3, (merge r2 r4, f2), d2)) (r := r)
+      in H13; eauto.
+    simpljoin1.
+    destruct_state x0.
+    simpl in H19.
+    simpljoin1.
+    eapply program_step_deterministic in H7; eauto.
+    simpljoin1.
+    eapply program_step_deterministic in H8; eauto.
+    simpljoin1.
+    exists I' (p' ** r).
+    repeat (split; eauto).
+    eapply Seq_frame_rule; eauto.
+    clear - H19 H21 H20 H15.
+    simpl.
+    do 2 eexists.
+    repeat (split; eauto).
+    simpl; eauto.
+    simpl; eauto.
+
+  -
+    simpl in H1.
+    simpljoin1.
+    eapply H0 in H1; eauto.
+
+  -
+    eapply H0 in H2.
+    eapply IHwf_seq in H2; eauto.
+    simpljoin1.
+    eapply Seq_conseq_rule in H2; eauto.
+Qed.
+
+Lemma bne_preservation :
+  forall p q S S1 S2 aexp pc npc pc1 npc1 pc2 npc2 Spec Spec' C i I,
+     wf_seq Spec p I q -> LookupC C pc npc I -> S |= p ->
+     wf_cdhp Spec C Spec' -> cdhp_subst Spec Spec' ->
+     C pc = Some (cbne aexp) -> C npc = Some (cntrans i) ->
+     P__ C (S, pc, npc) (S1, pc1, npc1) -> P__ C (S1, pc1, npc1) (S2, pc2, npc2) ->
+     exists I' p',
+       wf_seq Spec p' I' q /\ LookupC C pc2 npc2 I' /\ S2 |= p'.
+Proof.
+  intros.
+  generalize dependent C.
+  generalize dependent S.
+  generalize dependent S1.
+  generalize dependent S2.
+  generalize dependent aexp.
+  generalize dependent pc.
+  generalize dependent pc1.
+  generalize dependent pc2.
+  generalize dependent npc.
+  generalize dependent npc1.
+  generalize dependent npc2.
+  generalize dependent i.
+ 
+  induction H; intros; elim_ins_neq.
+ 
+  -
+    inversion H12; subst.
+    rewrite H10 in H20.
+    inversion H20; subst.
+    inversion H25; get_ins_diff_false.
+
+    clear H23 H20 H21.
+    eapply dly_reduce_asrt_stable in H17; eauto.
+    lets Haexp : H17.
+    eapply H in Haexp.
+    simpl in Haexp.
+    simpljoin1.
+    rewrite H33 in H14.
+    inversion H14; subst.
+    clear H14 H15.
+    assert (bv = $ 0).
+    {
+      clear - H2 H34 H17.
+      eapply H2 in H17.
+      sep_star_split_tac.
+      simpls.
+      simpljoin1.
+      clear H2.
+      unfolds regSt.
+      simpls.
+      simpljoin1.
+      unfold merge in *.
+      unfolds RegMap.set.
+      destruct_rneq_H.
+      inversion H34; eauto.
+    }
+
+    subst.
+    inversion H13; subst.
+    eapply dly_reduce_asrt_stable in H18; eauto.
+    inversion H28; get_ins_diff_false.
+    eapply ins_rule_sound in H1.
+    eapply total_to_partial in H1.
+    eapply H1 in H18; eauto.
+    eapply H18 in H26; eauto.
+    clear H18.
+    assert (($ 0) =ᵢ ($ 0) = true).
+    {
+      eapply Int.eq_true; eauto.
+    }
+    eapply H6 in H14; eauto.
+    unfold wf_cdhp in H9.
+    unfold cdhp_subst in H3.
+    eapply H3 in H0; eauto.
+    eapply H9 with (L := L) in H0; eauto.
+    simpljoin1.
+    renames x to I'.
+    exists I' p'.
+    repeat (split; eauto).
+    eapply Seq_frame_rule in H16; eauto.
+    clear - H16 H14 H15.
+    eapply Seq_conseq_rule; eauto.
+
+    clear H20 H23 H22.
+    eapply dly_reduce_asrt_stable in H17; eauto.
+    assert (bv = v).
+    {
+      clear - H2 H34 H17.
+      eapply H2 in H17.
+      sep_star_split_tac.
+      simpls.
+      simpljoin1.
+      unfolds regSt.
+      simpls.
+      simpljoin1.
+      unfold merge in *.
+      unfolds RegMap.set.
+      destruct_rneq_H.
+      inversion H34; eauto.
+    }
+    subst.
+    inversion H13; subst.
+    eapply dly_reduce_asrt_stable in H17; eauto.
+    eapply ins_rule_sound in H1.
+    eapply total_to_partial in H1.
+    inversion H28; get_ins_diff_false.
+    eapply H1 in H17; eauto.
+    eapply H17 in H26; eauto.
+    clear H17.
+    exists I (p' //\\ [|v =ᵢ ($ 0) = false|]).
+    repeat (split; eauto).
+    clear - H24.
+    assert ((pc1 +ᵢ ($ 4)) +ᵢ ($ 4) = pc1 +ᵢ ($ 8)).
+    {
+      rewrite Int.add_assoc.
+      simpl; eauto.
+    }
+    rewrite H; eauto.
+    clear - H35.
+    simpl.
+    unfold Int.eq.
+    destruct (zeq (Int.unsigned v) (Int.unsigned $ 0)); eauto.
+    eapply z_eq_to_int_eq in e.
+    do 2 rewrite Int.repr_unsigned in e.
+    subst.
+    tryfalse.
     
+  - 
+    rewrite H5 in H9.
+    inversion H9; subst.
+    clear H9 H10.
+    sep_star_split_tac.
+    simpl in H13.
+    simpljoin1.
+    eapply bne_progress in H; eauto.
+    simpljoin1.
+    destruct_state x.
+    destruct_state x0.
+    eapply IHwf_seq in H1; eauto.
+    destruct H1 as [ I' [p' H1] ].
+    simpljoin1. 
+    eapply program_step_safety_property with (s := (merge m m0, (merge r0 r1, f0), d0)) (r := r)
+      in H; eauto.
+    simpljoin1.
+    destruct_state x0.
+    simpl in H16.
+    simpljoin1.
+    eapply program_step_safety_property with (s := (merge m1 m3, (merge r2 r4, f2), d2)) (r := r)
+      in H13; eauto.
+    simpljoin1.
+    destruct_state x0.
+    simpl in H19.
+    simpljoin1.
+    eapply program_step_deterministic in H7; eauto.
+    simpljoin1.
+    eapply program_step_deterministic in H8; eauto.
+    simpljoin1.
+    exists I' (p' ** r).
+    repeat (split; eauto).
+    eapply Seq_frame_rule; eauto.
+    clear - H19 H21 H20 H15.
+    simpl.
+    do 2 eexists.
+    repeat (split; eauto).
+    simpl; eauto.
+    simpl; eauto.
+
+  -
+    simpl in H1.
+    simpljoin1.
+    eapply H0 in H1; eauto.
+
+  -
+    eapply H0 in H2.
+    eapply IHwf_seq in H2; eauto.
+    simpljoin1.
+    eapply Seq_conseq_rule in H2; eauto.
+Qed.
+
+Lemma retl_preservation :
+  forall p q Spec S S1 S2 pc npc pc1 npc1 pc2 npc2 C I,
+    wf_seq Spec p I q -> LookupC C pc npc I -> S |= p -> C pc = Some cretl ->
+    P__ C (S, pc, npc) (S1, pc1, npc1) -> P__ C (S1, pc1, npc1) (S2, pc2, npc2) ->
+    S2 |= q.
+Proof.
+  intros.
+  generalize dependent S.
+  generalize dependent S1.
+  generalize dependent S2.
+  generalize dependent C.
+  generalize dependent pc1.
+  generalize dependent npc1.
+  generalize dependent pc2.
+  generalize dependent npc2.
+ 
+  induction H; intros; elim_ins_neq.
+
+  -
+    clear H12.
+    inversion H2; get_ins_diff_false.
+    clear H8 H12.
+    inversion H6; subst.
+    inversion H16; get_ins_diff_false.
+    clear H11. 
+    eapply dly_reduce_asrt_stable in H10; eauto.
+    inversion H4; subst.
+    inversion H21; get_ins_diff_false.
+    eapply dly_reduce_asrt_stable in H11; eauto.
+    eapply ins_rule_sound in H.
+    eapply total_to_partial in H.
+    eapply H in H11; eauto.
+
+  -
+    sep_star_split_tac.
+    simpl in H11.
+    simpljoin1.
+    eapply retl_progress in H; eauto.
+    simpljoin1.
+    destruct_state x.
+    destruct_state x0.
+    eapply IHwf_seq in H3; eauto.
+    eapply program_step_safety_property with (s := (merge m m0, (merge r0 r1, f0), d0))
+      (r := r) in H; eauto.
+    simpljoin1.
+    destruct_state x0.
+    simpls.
+    simpljoin1.
+    eapply program_step_safety_property with (s := (merge m1 m3, (merge r2 r4, f2), d2))
+       (r := r) in H9; eauto.
+    simpljoin1.
+    destruct_state x0.
+    simpl in H14.
+    simpljoin1.
+    eapply program_step_deterministic in H5; eauto.
+    simpljoin1.
+    eapply program_step_deterministic in H4; eauto.
+    simpljoin1.
+    exists (m2, (r3, f), d) (m4, (r5, f), d).
+    simpl; eauto. 
+    repeat (split; eauto).
+    simpl; eauto.
+    simpl; eauto.
+
+  -
+    simpls.
+    simpljoin1; eauto.
+
+  -
+    eapply H0 in H5.
+    eauto.
+Qed.
+
+Lemma call_preservation :
+  forall p q Spec Spec' f S S1 S2 pc pc1 pc2 npc npc1 npc2 C I,
+    wf_seq Spec p I q -> LookupC C pc npc I -> S |= p ->
+    wf_cdhp Spec C Spec' -> cdhp_subst Spec Spec' ->
+    C pc = Some (ccall f) ->
+    P__ C (S, pc, npc) (S1, pc1, npc1) -> P__ C (S1, pc1, npc1) (S2, pc2, npc2) ->
+    exists I1 I2 p1 p2,
+      wf_seq Spec p1 I1 p2 /\ LookupC C pc2 npc2 I1 /\ S2 |= p1 /\ p2 ==> Or r15 ==ₑ pc /\ 
+      wf_seq Spec p2 I2 q /\ LookupC C (pc +ᵢ ($ 8)) (pc +ᵢ ($ 12)) I2.
+Proof.
+  intros.
+  generalize dependent S.
+  generalize dependent S1.
+  generalize dependent S2.
+  generalize dependent C.
+  generalize dependent pc1.
+  generalize dependent npc1.
+  generalize dependent pc2.
+  generalize dependent npc2.
+  generalize dependent f.
+ 
+  induction H; intros; elim_ins_neq.
+ 
+  -
+    clear H22.
+    inversion H14; subst.
+    eapply dly_reduce_asrt_stable in H18; eauto.
+    eapply H0 in H18.
+    inversion H23; get_ins_diff_false.
+    clear H20. 
+    assert ((M', (set_R R' r15 f1, F'), D'') |= r15 |=> f1 ** p1).
+    {
+      clear - H18.
+      sep_star_split_tac.
+      simpl in H3.
+      simpljoin1.
+      simpl.
+      exists (m, (set_R r r15 f1, f0), d0) (m0, (r0, f0), d0).
+      simpls.
+      unfolds regSt.
+      simpls.
+      simpljoin1.
+      repeat (split; eauto).
+      eapply disjoint_setR_still1; eauto.
+      rewrite indom_setR_merge_eq1; eauto.
+      eapply regset_l_l_indom; eauto.
+      rewrite indom_setR_eq_RegMap_set; eauto.
+      rewrite regset_twice; eauto.
+      eapply regset_l_l_indom; eauto.
+    } 
+    inversion H12; subst.
+    eapply dly_reduce_asrt_stable in H20; eauto.
+    eapply ins_rule_sound in H1.
+    eapply total_to_partial in H1; eauto.
+    inversion H31; get_ins_diff_false.
+    eapply H1 in H20; eauto.
+    eapply H20 in H29; eauto.
+    clear H20.
+    unfold cdhp_subst in H3.
+    unfold wf_cdhp in H10. 
+    eapply H3 in H.
+    eapply H10 with (L := L) in H.
+    simpljoin1.
+    rename x into I'.
+    eapply Seq_frame_rule with (r := r) in H16; eauto.
+    exists I' I (fp L ** r) (fq L ** r).
+    repeat (split; eauto).
+    clear - H6.
+    intros.
+    sep_star_split_tac.
+    simpl in H3.
+    simpljoin1.
+    eapply H6 in H; eauto.
+    clear - H.
+    simpls.
+    unfold merge.
+    rewrite H; eauto.
+    eapply Seq_conseq_rule; eauto.
+    clear - H26.
+    do 2 rewrite Int.add_assoc in H26.
+    simpls; eauto.
+
+  -
+    sep_star_split_tac.
+    simpls.
+    simpljoin1.
+    eapply call_progress in H; eauto.
+    simpljoin1.
+    destruct_state x.
+    destruct_state x0.
+    eapply IHwf_seq in H5; eauto.
+    simpljoin1.   
+    eapply program_step_safety_property with (s := (merge m m0, (merge r0 r1, f1), d0)) (r := r)
+      in H; eauto. 
+    simpljoin1.
+    destruct_state x8.
+    simpls.
+    simpljoin1.
+    eapply program_step_safety_property with (s := (merge m1 m3, (merge r2 r4, f3), d2)) (r := r)
+      in H12; eauto.
+    simpljoin1.
+    eapply program_step_deterministic in H7; eauto.
+    simpljoin1.
+    eapply program_step_deterministic in H6; eauto.
+    destruct_state x8.
+    simpls.
+    simpljoin1. 
+    exists x x0 (x5 ** r) (x6 ** r).
+    repeat (split; eauto).
+    eapply Seq_frame_rule; eauto.
+    simpl.
+    do 2 eexists.
+    repeat (split; eauto).
+    clear - H16.
+    intros.
+    sep_star_split_tac.
+    simpls.
+    simpljoin1.
+    simpls.
+    eapply H16 in H.
+    simpls.
+    unfold merge.
+    rewrite H; eauto.
+    eapply Seq_frame_rule; eauto.
+    simpl; eauto.
+    simpl; eauto.
+
+  -
+    simpls.
+    simpljoin1; eauto.
+
+  -
+    eapply H0 in H7. 
+    eapply IHwf_seq with (pc2 := pc2) (npc2 := npc2) in H7; eauto.
+    simpljoin1.
+    exists x x0 x1 x2; eauto.
+    repeat (split; eauto).
+    eapply Seq_conseq_rule; eauto.
+Qed.
+    
+(*+ Lemmas for Sequence Rule +*)
     
 Lemma program_step_next :
   forall C S S' pc npc pc' npc',
@@ -1727,7 +2628,24 @@ Proof.
   inversion H; subst.
   inversion H8; subst; eauto.
 Qed.
+
+Lemma insSeq_rule_sound :
+  forall cls Spec Spec' p q I pc npc S C,
+    wf_seq Spec p I q -> LookupC C pc npc I ->
+    wf_cdhp Spec C Spec' -> cdhp_subst Spec Spec' -> S |= p ->
+    safety_step C S pc npc q cls 0.
+Proof.
+  intro cls.
+  induction cls; intros.
+  -
+    eapply safety_step_ret1; intros.
+    eapply retl_preservation in H; eauto.
+  -
+    
   
+
+>>>>>>>>>>>>>>>>>>>>>
+    
 Lemma insSeq_rule_sound :
   forall Spec Spec' p q I pc npc S C,
     wf_seq Spec p I q -> LookupC C pc npc I ->
@@ -1784,579 +2702,42 @@ Proof.
     rewrite Hnpc in H5.
     inversion H5; subst.
     clear H5.
+    eapply be_preservation in H; eauto.
+    simpljoin1.
+    renames x0 to p', x to I'.
+    eauto.
+
+  - (** C pc = bne aexp *)
+    lets Hnpc : H4.
+    eapply pc_bne_npc_i in Hnpc; eauto.
+    destruct Hnpc as [i Hnpc].
+    lets Ht : H5.
+    eapply program_step_next in H5.
+    subst.
+    eapply safety_cons;
+      try solve [intros; get_ins_diff_false].
+    intros.
+    rewrite Hnpc in H5.
+    inversion H5; subst.
+    clear H5.
+    eapply bne_preservation in H; eauto.
+    simpljoin1.
+    renames x0 to p', x to I'.
+    eauto.
+
+  - (** C pc = call f *)  
+    eapply call_preservation in H; eauto.
+    simpljoin1. 
+    renames x1 to p1, x2 to p2, x to Ic, x0 to I'.
+    admit.
+    
+  - (** retl *)
+    left.
+    split; eauto.
+    eapply retl_preservation; eauto.
     
     
     >>>>>>>>>>>>>>>>>
-    
-  
-  
-  cofix.
-  intros.
-  inversion H; subst.
- 
-  - (** Seq *)
-    inversion H0; subst.
-    clear H.
-    eapply safety_cons;
-      try solve [intros; get_ins_diff_false].
-    intros.
-    rewrite H11 in H.
-    inversion H; subst.
-    clear H.
-    inversion H6; subst.
-    eapply ins_rule_sound in H4.
-    eapply total_to_partial in H4; eauto.
-    inversion H16; get_ins_diff_false.
-    eapply dly_reduce_asrt_stable in H3; eauto.
-
-  - (** Call *)
-    eapply call_test.
-
-  - (** retl *)
-    clear H.
-    inversion H0; subst.
-    eapply safety_cons;
-      try solve [intros; get_ins_diff_false].
-    intros.
-    left.
-    inversion H7; subst.
-    clear H11.
-    inversion H19; get_ins_diff_false.
-    eapply dly_reduce_asrt_stable in H3; eauto.
-    clear H14.
-    inversion H8; subst.
-    eapply dly_reduce_asrt_stable in H3; eauto.
-    inversion H23; get_ins_diff_false.
-    eapply ins_rule_sound in H4.
-    eapply total_to_partial in H4.
-    eapply H4 in H3; eauto.
-
-  - (** J1 *)
-    
-    clear H.
-    inversion H0; subst.
-    eapply safety_cons;
-      try solve [intros; get_ins_diff_false].
-    intros.
-    inversion H11; subst.
-    eapply dly_reduce_asrt_stable in H3; eauto.
-    inversion H22; get_ins_diff_false.
-    rewrite H15 in H.
-    inversion H; subst.
-    clear H15 H21.
-    lets Hp : H3.
-    eapply H4 in Hp.
-    simpl in Hp.
-    simpljoin1.
-    rewrite H30 in H12.
-    inversion H12; subst.
-    clear H12.
-    eapply safety_cons;
-      try solve [intros; get_ins_diff_false].
-    intros.
-    inversion H12; subst.
-    inversion H28; get_ins_diff_false.
-    clear H20 H12 H28.
-    lets Ht : H3.
-    eapply H6 in Ht.
-    eapply sep_star_split in Ht.
-    destruct Ht as [ s1 [s2 [Hs1 [Hs2 Hunion] ] ] ].
-    destruct_state s1.
-    destruct_state s2.
-    simpl in Hunion.
-    simpljoin1.
-    rename pc'0 into f.
-
-    assert (Hset_rd : (m, (set_R r0 rd0 f1, f0), d0) |= rd0 |=> f1).
-    {
-      clear - Hs1.
-      simpls.
-      unfolds regSt.
-      simpls.
-      simpljoin1.
-      repeat (split; eauto).
-      rewrite indom_setR_eq_RegMap_set; eauto.
-      rewrite regset_twice; eauto.
-      eapply regset_l_l_indom; eauto.
-    }
-
-    assert (Hset_rd_asrt :
-              (merge m m0, (merge (set_R r0 rd0 f1) r1, f0), d0) |= rd0 |=> f1 ** p1).
-    {
-      clear - Hset_rd H12 H14 Hs1 Hs2.
-      simpls.
-      exists (m, (set_R r0 rd0 f1, f0), d0) (m0, (r1, f0), d0).
-      simpl.
-      repeat (split; eauto).
-      eapply disjoint_setR_still1; eauto.
-    }
-    rewrite <- indom_setR_merge_eq1 in Hset_rd_asrt; eauto.
-    eapply ins_rule_sound in H7.
-    eapply total_to_partial in H7.
-    eapply dly_reduce_asrt_stable in Hset_rd_asrt; eauto.
-    rewrite H19 in H.
-    inversion H; subst.
-    eapply H7 in Hset_rd_asrt; eauto.
-    eapply Hset_rd_asrt in H26; eauto.  
-    clear - insSeq_rule_sound H1 H2 H5 H26 H8 H9 H10.
-    lets Hwfcdhp : H1.
-    lets Hcdhpsubst : H2.
-    unfold wf_cdhp in H1.
-    unfold cdhp_subst in H2.
-    eapply H2 in H5; eauto.
-    eapply H1 with (L := L) in H5.
-    simpljoin1.
-    rename x into I.
-    eapply H8 in H26.
-    eapply Seq_frame_rule with (r := r) in H0; eauto.
-    clear H1 H2.
-    eapply insSeq_rule_sound in H0; eauto.
-    eapply safety_post_weak in H0; eauto.
-    clear - Hset_rd.
-    simpls.
-    unfolds regSt.
-    simpls.
-    simpljoin1.
-    unfolds set_R.
-    unfold is_indom in *.
-    destruct (r0 rd0) eqn:Heqe; tryfalse.
-    unfold indom; eauto.
-    subst.
-    unfolds RegMap.set.
-    destruct_rneq_H.
-
-  - (** J2 *)
-    eapply call_test.
-    
-    (*
-    inversion H0; subst.
-    eapply safety_cons;
-      try solve [intros; get_ins_diff_false].
-    intros.
-    rewrite H17 in H12.
-    inversion H12; subst.
-    inversion H13; subst.
-    lets Hp : H3.
-    eapply dly_reduce_asrt_stable in Hp; eauto.
-    clear H18 H13.
-    inversion H24; get_ins_diff_false.
-    lets Hf1 : Hp.
-    eapply H4 in Hf1; eauto.
-    simpl in Hf1.
-    simpljoin1.
-    rewrite H30 in H13.
-    inversion H13; subst.
-    clear H13.
-    lets Hrd : Hp.
-    eapply H5 in Hrd; eauto.
-    assert ((M', (set_R R' rd0 f1, F'), D'') |= rd0 |=> f1 ** p1).
-    {
-      clear - Hrd.
-      sep_star_split_tac.
-      simpl in H3.
-      simpljoin1.
-      simpl.
-      exists (m, (set_R r rd0 f1, f0), d0) (m0, (r0, f0), d0).
-      simpls.
-      repeat (split; eauto).
-      eapply disjoint_setR_still1; eauto.
-      rewrite indom_setR_merge_eq1; eauto.
-      clear - H1.
-      unfolds regSt.
-      simpls.
-      simpljoin1.
-      eapply regset_l_l_indom; eauto.
-      simpls.
-      rewrite indom_setR_eq_RegMap_set; eauto.
-      unfolds regSt.
-      simpls.
-      simpljoin1.
-      rewrite regset_twice; eauto.
-      unfolds regSt.
-      simpls.
-      simpljoin1.
-      eapply regset_l_l_indom; eauto.
-      simpl; eauto.
-      unfolds regSt.
-      simpls.
-      simpljoin1; eauto.
-    }
-    
-    eapply safety_cons;
-      try solve [intros; get_ins_diff_false].
-    intros.
-    rewrite H22 in H13.
-    inversion H13; subst.
-    inversion H15; subst.
-    clear H15.
-    eapply dly_reduce_asrt_stable in H12; eauto.
-    lets Hp' : H12.
-    eapply H7 in H12.
-    inversion H33; get_ins_diff_false.
-    eapply H6 in Hp'.
-    simpl in Hp'.
-    simpljoin1. 
-    clear H20.
-    rewrite H15 in H37.
-    inversion H37; subst; eauto.
-
-    assert ((M'0, (set_R R'0 rd1 pc', F'0), D''0) |= rd1 |=> pc' ** p2).
-    {
-      clear - H12.
-      sep_star_split_tac.
-      simpl in H3.
-      simpljoin1.
-      simpls.
-      unfolds regSt.
-      simpls.
-      simpljoin1.
-      exists (empM, (set_R (RegMap.set rd1 (Some v2) empR) rd1 pc', f0), d0)
-        (m0, (r0, f0), d0).
-      simpl.
-      repeat (split; eauto).
-      eapply disjoint_setR_still1; eauto. 
-      rewrite indom_setR_merge_eq1; eauto.
-      eapply regset_l_l_indom; eauto.
-      rewrite indom_setR_eq_RegMap_set; eauto.
-      rewrite regset_twice; eauto.
-      eapply regset_l_l_indom; eauto.
-    }
-
-    eapply H9 in H13.   
-    clear - insSeq_rule_sound H1 H2 H8 H10 H13 H11.
-    lets Hwfcdhp : H1.
-    unfold wf_cdhp in H1.
-    lets Hcdhpsubset : H2.
-    unfold cdhp_subst in H2.
-    eapply H2 in H8.
-    eapply H1 with (L := L) in H8; eauto.
-    simpljoin1.
-    rename x into I. 
-    eapply Seq_frame_rule with (r := r) in H0; eauto.
-    eapply insSeq_rule_sound in H0; eauto.
-    eapply safety_post_weak in H0; eauto. *)
-
-  - (** be *)
-    
-    inversion H0; subst.
-    eapply safety_cons;
-      try solve [intros; get_ins_diff_false].
-    clear H H0.
-    intros.
-    rewrite H17 in H.
-    inversion H; subst.
-    inversion H0; subst.
-    eapply dly_reduce_asrt_stable in H14; eauto.
-    lets Hp1 : H14.
-    eapply H4 in Hp1; eauto.  
-    inversion H22; get_ins_diff_false.
-
-    eapply call_test.
-    (*
-    simpl in Hp1.
-    simpljoin1.  
-    rewrite H11 in H30.
-    inversion H30; subst.
-    clear H30 H17. 
-    
-    assert (v = bv).
-    {
-      clear - H7 H14 H31.
-      eapply H7 in H14.
-      sep_star_split_tac.
-      simpl in H3.
-      simpljoin1.
-      clear - H1 H31.
-      simpl in H1.
-      unfolds regSt.
-      simpls.
-      simpljoin1.
-      unfolds RegMap.set.
-      unfold merge in *.
-      destruct_rneq_H.
-      inversion H31; subst; eauto.
-    }
-
-    subst v.
-    eapply safety_cons;
-      try solve [intros; get_ins_diff_false].
-    intros.
-    rewrite H20 in H.
-    inversion H; subst.
-    clear H.
-    inversion H13; subst.
-    inversion H28; get_ins_diff_false.
-    eapply dly_reduce_asrt_stable in H17; eauto.
-    eapply ins_rule_sound in H6.
-    eapply total_to_partial in H6.
-    eapply H6 in H17; eauto.
-    eapply H17 in H26; eauto.
-    clear H17 H18.   
-    clear - insSeq_rule_sound H5 H9 H10 H32 H26 H1 H2 H21.
-    assert (Hbv_false : bv =ᵢ ($ 0) = false).
-    {
-      clear - H32.
-      unfold Int.eq.
-      destruct (zeq (Int.unsigned bv) (Int.unsigned $ 0)); eauto.
-      {
-        eapply z_eq_to_int_eq in e.
-        rewrite Int.repr_unsigned in e.
-        rewrite Int.repr_unsigned in e.
-        subst.
-        tryfalse.
-      }
-    }
-    eapply H10 in Hbv_false.
-    simpljoin1.
-    lets Hwfcdhp : H1.
-    lets Hcdhpsubst : H2.
-    unfold wf_cdhp in H1.
-    unfold cdhp_subst in H2.
-    eapply H2 in H5.
-    eapply H1 with (L := L) in H5.
-    simpljoin1.
-    rename x into I.
-    eapply H in H26.
-    eapply Seq_frame_rule with (r := r) in H4; eauto.
-    eapply insSeq_rule_sound in H4; eauto.
-    eapply safety_post_weak; eauto.
-*)
-
-    clear H17.
-    eapply safety_cons;
-      try solve [intros; get_ins_diff_false].
-    intros.
-    rewrite H20 in H11. 
-    inversion H11; subst.
-    clear H11.
-    inversion H12; subst.
-    lets Hp' : H14.
-    eapply dly_reduce_asrt_stable in Hp'; eauto.
-    inversion H28; get_ins_diff_false.
-    lets Hp1' : H14.
-    simpl in Hp1.
-    simpljoin1.
-    rewrite H11 in H30.
-    inversion H30; subst.
-    eapply ins_rule_sound in H6.
-    eapply total_to_partial in H6.
-    eapply H6 in Hp'; eauto.
-    eapply Hp' in H26; eauto. 
-    clear Hp'.
-    assert (bv =ᵢ ($ 0) = true).
-    {
-      eapply H7 in H14.
-      clear - H14 H31.
-      sep_star_split_tac.
-      simpl in H1.
-      simpl in H3.
-      simpljoin1.
-      unfolds regSt.
-      simpls.
-      simpljoin1.
-      clear - H31.
-      unfolds RegMap.set.
-      unfold merge in *.
-      destruct_rneq_H.
-      inversion H31.
-      unfold Int.eq.
-      assert (Int.unsigned Int.zero = 0%Z).
-      eapply Int.unsigned_zero; eauto.
-      unfold Int.zero in H0.
-      rewrite H0; eauto.
-    }
-    clear - insSeq_rule_sound H1 H2 H8 H21 H26 H.
-    eapply insSeq_rule_sound in H8; eauto.
-    assert (pc' +ᵢ ($ 8) = (pc' +ᵢ ($ 4)) +ᵢ ($ 4)).
-    {
-      rewrite Int.add_assoc.
-      assert ($ 8 = ($ 4) +ᵢ ($ 4)).
-      eauto.
-      rewrite <- H0.
-      eauto.
-    }
-    rewrite <- H0.
-    eauto.
-    simpl; eauto.
-
-  - (** Bne *)
-    eapply call_test.
-    
-  (*
-    clear H.
-    inversion H0; subst.
-    eapply safety_cons;
-      try solve [intros; get_ins_diff_false].
-    intros.
-    inversion H11; subst.
-    clear H11.
-    eapply dly_reduce_asrt_stable in H15; eauto.
-    lets Hp1 : H15.
-    eapply H4 in H15.
-    simpl in H15. 
-    simpljoin1.
-    inversion H23; get_ins_diff_false.
-    rewrite H16 in H.
-    inversion H; subst.
-    rewrite H11 in H31.
-    inversion H31; subst.
-    clear H31 H21 H H16.
-    assert (bv = $ 0).
-    {
-      clear - Hp1 H32 H7.
-      eapply H7 in Hp1.
-      sep_star_split_tac.
-      simpl in H3.
-      simpljoin1.
-      simpl in H1.
-      unfolds regSt.
-      simpls.
-      simpljoin1.
-      unfold merge in H32.
-      unfolds RegMap.set.
-      destruct_rneq_H.
-      inversion H32; eauto.
-    }
-    subst.
-    eapply safety_cons;
-      try solve [intros; get_ins_diff_false].
-    intros.
-    rewrite H19 in H.
-    inversion H; subst.
-    clear H.
-    inversion H13; subst.
-    eapply dly_reduce_asrt_stable in H16; eauto.
-    eapply ins_rule_sound in H6.
-    eapply total_to_partial in H6; eauto.
-    inversion H27; get_ins_diff_false.
-    eapply H6 in H16; eauto.
-    eapply H16 in H25; eauto.
-    clear H16. 
-    clear - insSeq_rule_sound H1 H2 H5 H25 H10 H9.
-    lets Hwfcdhp : H1.
-    lets Hcdhpsubset : H2.
-    unfold wf_cdhp in H1.
-    unfold cdhp_subst in H2.
-    eapply H2 in H5.
-    eapply H1 with (L := L) in H5; eauto.
-    assert (($ 0) =ᵢ ($ 0) = true).
-    {
-      rewrite Int.eq_true; eauto.
-    } 
-    eapply H10 in H.
-    simpljoin1.
-    eapply H in H25; eauto.
-    eapply Seq_frame_rule with (r := r) in H4; eauto.
-    eapply insSeq_rule_sound in H4; eauto.
-    eapply safety_post_weak; eauto.
-
-    rewrite H16 in H.
-    inversion H; subst.
-    clear H16.
-    eapply safety_cons;
-      try solve [intros; get_ins_diff_false].
-    intros.
-    inversion H14; subst.
-    eapply dly_reduce_asrt_stable in H18; eauto.
-    eapply ins_rule_sound in H6.
-    eapply total_to_partial in H6.
-    inversion H30; get_ins_diff_false.
-    rewrite H19 in H13.
-    inversion H13; subst.
-    clear H19 H21 H13.
-    eapply H6 in H18; eauto.
-    eapply H18 in H28; eauto.
-    clear H18.
-    assert (bv = v).
-    {
-      clear - H7 Hp1 H32.
-      eapply H7 in Hp1; eauto.
-      sep_star_split_tac.
-      simpl in H3.
-      simpljoin1.
-      simpl in H1.
-      unfolds regSt.
-      simpls.
-      simpljoin1.
-      unfold merge in H32.
-      unfolds RegMap.set.
-      destruct_rneq_H.
-      inversion H32; eauto.
-    }
-    subst.
-    clear - insSeq_rule_sound H1 H2 H5 H8 H28 H20 H33.
-    eapply insSeq_rule_sound in H8; eauto.
-    assert (pc' +ᵢ ($ 8) = (pc' +ᵢ ($ 4)) +ᵢ ($ 4)).
-    {
-      rewrite Int.add_assoc; eauto.
-    }
-    rewrite <- H.
-    eauto.
-    simpl.
-    split; eauto.
-    clear - H33.
-    unfold Int.eq.
-    destruct (zeq (Int.unsigned v) (Int.unsigned $ 0)) eqn:Heqe; eauto.
-    clear Heqe.
-    eapply z_eq_to_int_eq in e.
-    do 2 rewrite Int.repr_unsigned in e.
-    subst.
-    tryfalse.
-*)
-
-  - (** frame *)
-    eapply call_test.
- 
-  - (** ex_intro *)
-    eapply call_test.
-    (*
-    clear H.
-    simpl in H3.
-    simpljoin1.
-    specialize (H4 x).
-    eapply insSeq_rule_sound in H4; eauto.*)
-Qed.
-
-
-    
-  - (** Seq *)
-    inversion H4; subst.
-    eapply safety_cons;
-      try solve [intros; get_ins_diff_false].
-    intros.
-
-    inversion H6; subst.
-    inversion H17; get_ins_diff_false.
-    rewrite H10 in H5; inversion H5; subst.
-    eapply ins_rule_sound in H.
-    eapply total_to_partial in H.
-    eapply dly_reduce_asrt_stable in H3; eauto.
-
-  - (** Call *)
-    admit.
-
-  - (** retl *)
-    inversion H5; subst.
-    eapply safety_cons;
-      try solve [intros; get_ins_diff_false].
-    intros.
-
-    left.
-    inversion H7; subst.
-    inversion H19; get_ins_diff_false.
-    eapply dly_reduce_asrt_stable in H4; eauto.
-    clear H11 H14 H15.
-    inversion H8; subst.
-    inversion H22; get_ins_diff_false.
-    eapply ins_rule_sound in H.
-    eapply total_to_partial in H; eauto.
-    eapply dly_reduce_asrt_stable in H4; eauto.
-
-  - (** jumpl *)
-    inversion H9; subst.
-    
-    
-    >>>>>>>>>>>>>>>>
     
   
 Theorem cdhp_rule_sound :
